live proc attempt

lemma/live_proc.v
@@ -1,4 +1,3 @@
-From mathcomp Require Import ssreflect.seq all_ssreflect.
 Require Import List String Coq.Arith.PeanoNat Coq.Program.Equality Relations ZArith Datatypes Setoid Morphisms Coq.Logic.Decidable Coq.Program.Basics Coq.Init.Datatypes Coq.Logic.Classical_Prop.
 Import ListNotations. 
 Open Scope list_scope.
@@ -7,13 +6,18 @@ Import ListNotations.
 From SST Require Import src.header src.sim src.expr src.process src.local 
 src.global src.balanced src.typecheck src.part src.gttreeh src.path_props src.step src.merge src.projection src.session src.lcontext.  
 From SST Require Import lemma.inversion lemma.path_assoc lemma.inversion_expr lemma.completeness lemma.substitution_helper lemma.substitution lemma.decidable_helper lemma.decidable lemma.expr lemma.part lemma.step 
-lemma.projection_helper lemma.subj_red_prog_fid lemma.projection lemma.subj_red_helpers lemma.soundness lemma.liveness_helpers.
+lemma.projection_helper lemma.subj_red_prog_fid lemma.projection lemma.subj_red_helpers lemma.soundness 
+lemma.liveness_helpers lemma.liveness.
+
+Definition typable M := exists gamma, typ_sess M gamma. 
 
 Definition proc_path_valid_criteria := (fun x1 (l:label)  x2  =>
   match (x1,l,x2) with 
-    | (g1,(lcomm p q ell), g2) => betaP_lbl g1 (lcomm p q ell) g2 
+    | (g1,(lcomm p q ell), g2) => betaP_lbl g1 (lcomm p q ell) g2 /\ typable g1
     | _=> False
   end).
+
+  From Coq Require Import IndefiniteDescription.
 
 Definition proc_valid_pathC := valid_path_GC proc_path_valid_criteria.
 
@@ -23,16 +27,495 @@ Print path_assoc.
 
 Search "local" "path".
 
-CoInductive typ_path  (R: coseq (session * option label) -> coseq (tctx * option label) -> Prop) :  coseq (session * option label) -> coseq (tctx * option label) -> Prop :=
+Variant typ_path  (R: coseq (session * option label) -> coseq (tctx * option label) -> Prop) :  coseq (session * option label) -> coseq (tctx * option label) -> Prop :=
     | typ_nil : typ_path R conil conil
-    | typ_cocons : forall M gamma ms gs l, typ_sess  M gamma -> typ_path R ms gs ->
+    | typ_cocons : forall M gamma ms gs l, typ_sess  M gamma ->  R ms gs ->
         typ_path R (cocons (M,l) ms) (cocons (gamma,l) gs).
 
-Definition live_sess Mp := forall M, betaRtc Mp M -> (forall p q ell e P' M', unfoldP M ( (p <-- p_send q ell e P') ||| M') -> exists M'',
+Definition gamma_by_betaP : forall M gamma p q ell M' l' xs, typ_sess M gamma -> proc_valid_pathC (cocons (M, Some (lcomm p q ell)) (cocons (M',l') xs)) ->
+{gamma' | typ_sess M' gamma' /\ tctxR gamma (lcomm p q ell) gamma' /\ proc_valid_pathC (cocons (M',l') xs)}.
+Proof.
+    intros * Htyp Hvalid.
+    assert(Hbeta: betaP_lbl M (lcomm p q ell) M').
+    {
+      pinversion Hvalid;try apply valid_path_mon;subst;red in H5;easy. 
+    }
+	Search betaP_lbl.
+	eapply sub_red_strong_labelled in Hbeta as Hsub;try exact Htyp.
+	destruct (constructive_indefinite_description _ Hsub) as [gamma' Hg'].
+    destruct Hg' as [Hassoc' Hstep].
+    exists gamma'. split;try easy. split;try easy.	
+	pinversion Hvalid;subst;try apply valid_path_mon. easy.
+Qed.
+
+CoFixpoint get_typ_path : forall M gamma l xs, typ_sess M gamma ->
+    proc_valid_pathC (cocons (M, l) xs) ->
+    local_path.
+Proof.
+    intros * Htyp Hvalid.
+    refine ((match l as m return 
+    (l =m -> local_path)
+    with 
+        | None =>  fun u=> (cocons (gamma, None) conil)
+        | Some (lcomm p q ell) => 
+        fun u=> (cocons (gamma,(Some (lcomm p q ell))) _)
+        | _ => fun u=> conil 
+    end
+    ) (eq_refl)).
+    {
+        destruct xs. exact conil.
+        subst. destruct p0. eapply gamma_by_betaP with (gamma:=gamma) in Hvalid;try easy.
+        destruct Hvalid as [gamma' [Hsess' [Hstep' Hvalid' ]]].
+        exact (get_typ_path s gamma' o xs Hsess'  Hvalid').
+    }
+Defined.
+
+
+Search path_assocC.
+
+Definition typ_pathC := paco2 typ_path bot2.
+
+Definition head_comm_enabled_proc p q ell (xs: coseq (session * option label)) := match xs with 
+  | cocons (M,_) xs => exists M', betaP_lbl M (lcomm p q ell) M'
+  | _ => False end.
+  
+Definition head_trans_proc p q ell (xs:coseq (session * option label)) := match xs with 
+  | cocons (_, Some (lcomm p' q' ell')) _ => p=p' /\ q=q' /\ ell =ell'
+  | _ => False end.
+
+Definition fairness_proc_inner xs := forall p q ell, head_comm_enabled_proc p q ell xs ->
+eventually (head_trans_proc p q ell) xs.
+
+Definition fair_path_proc := alwaysCG fairness_proc_inner.
+
+Lemma get_typ_path_types : forall M gamma l xs
+ (Htyp : typ_sess M gamma) 
+(Hvalid : proc_valid_pathC (cocons (M,l) xs)),
+typ_pathC (cocons (M,l) xs) 
+(get_typ_path _ _ _ _ Htyp Hvalid).
+Proof.
+    pcofix CIH.
+    intros.
+    destruct l.
+    {
+        
+        destruct l;
+        pose proof Hvalid as Hvalid'; pinversion Hvalid'; try apply valid_path_mon;try tauto;subst.
+
+        rewrite (coseq_eq (get_typ_path _ _ _ _ _ _   )).
+        simpl.
+        pfold.
+        constructor;try easy.
+        unfold eq_rect_r. simpl.
+		Check gamma_by_betaP.
+        set (gnext:= gamma_by_betaP M gamma n n0 n1 x l' xs0 Htyp  Hvalid).
+        destruct gnext.
+        destruct a. destr_hyps.
+        right. eapply CIH.            
+    }
+    {   
+        pose proof Hvalid as Hvalid'.
+        pinversion Hvalid';subst;try apply valid_path_mon;try easy. 
+        
+        rewrite (coseq_eq (get_typ_path _ _ _ _ _ _   )). simpl. 
+        pfold. constructor;try easy. left;pfold; constructor;try easy.
+    }
+Qed.
+
+Lemma get_typ_path_valid : forall M gamma l xs
+ (Htyp : typ_sess M gamma) 
+(Hvalid : proc_valid_pathC (cocons (M,l) xs)),
+local_valid_pathC  
+(get_typ_path _ _ _ _ Htyp Hvalid).
+Proof.
+    pcofix CIH.
+    intros.
+    destruct l.
+    {
+        
+        destruct l;
+        pose proof Hvalid as Hvalid'; pinversion Hvalid'; try apply valid_path_mon;try tauto;subst.
+        destruct l'.
+        {
+            destruct l;
+            pose proof H1 as Hvalid3;
+            pinversion Hvalid3;subst;try apply valid_path_mon;try easy.
+            rewrite (coseq_eq (get_typ_path _ _ _ _ _ _   )). simpl.
+            unfold eq_rect_r;simpl.   
+            set (gnext' := gamma_by_betaP M gamma n n0 n1 x (Some (lcomm n2 n3 n4))
+(cocons (x0, l') xs) Htyp Hvalid).
+            destruct gnext'. destr_hyps. pfold.
+            assert (Hfold: exists x2 w0 t1 , 
+			((get_typ_path x x1 (Some (lcomm n2 n3 n4)) (cocons (x0, l') xs) t p))
+			 = (cocons (x1, Some (lcomm n2 n3 n4)) (get_typ_path x0 x2 l' xs w0 t1 ))).
+            {
+                 rewrite (coseq_eq (get_typ_path _ _  _ _ _ _   )). simpl.
+            
+            unfold eq_rect_r. simpl.
+            set (gnext'' := gamma_by_betaP x x1 n2 n3 n4 x0 l' xs t p).
+            destruct gnext''. destr_hyps.
+            exists x2,  t1,  p0. easy.
+
+            }
+            destr_hyps.
+            rewrite H.
+            constructor;try solve [red;easy].
+            rewrite <- H.
+            right. eapply CIH.
+        }
+        rewrite (coseq_eq (get_typ_path _ _ _ _ _ _ )). simpl.
+        unfold eq_rect_r. simpl.
+        
+        set (gnext' := gamma_by_betaP M gamma n n0 n1 x None xs0 Htyp
+Hvalid).
+        destruct gnext';destr_hyps.
+        
+
+        rewrite (coseq_eq (get_typ_path _ _ _ _ _ _ )). simpl.
+        unfold eq_rec_r. simpl.
+        pfold. constructor. left. pfold. constructor.
+        red;easy.            
+    }
+    {   
+        pose proof Hvalid as Hvalid'.
+        pinversion Hvalid';subst;try apply valid_path_mon;try easy. 
+        
+        rewrite (coseq_eq (get_typ_path _ _ _ _ _ _   )). simpl. 
+        pfold. constructor;try easy. 
+    }
+Qed.
+
+Lemma typ_path_mon : monotone2 typ_path.
+Proof.
+	red;intros;induction IN;try constructor;try easy;eapply LE;easy.
+Qed.
+
+Hint Resolve typ_path_mon :paco.
+
+Lemma typ_path_preserves_fairness_helper : forall xs ys p q ell, typ_pathC xs ys -> eventually (head_trans_proc p q ell) xs ->
+eventually (headComm p q) ys.
+Proof.
+	intros * Htyp Hev. generalize dependent ys.
+	induction Hev;intros.
+	destruct xs;try easy. destruct p0. destruct o;try easy. destruct l;try easy. red in H;destr_hyps;subst.
+	pinversion Htyp;subst. constructor. simpl;tauto.
+	
+	pinversion Htyp;subst. specialize (IHHev _ H3). constructor 2. easy.
+Qed.
+	
+
+Lemma typ_path_preserves_fairness : forall xs ys, proc_valid_pathC xs -> fair_path_proc xs -> typ_pathC xs ys ->
+fair_path ys.
+Proof.
+	pcofix CIH.
+	intros * Hvalid Hfair Htyp. pfold. 
+	pinversion Htyp;subst. constructor. red;intros. inversion H.	
+	constructor. red;intros. simpl in H1. red in H1;destr_hyps.
+	eapply sess_fidelity in H1 as Hfid;try exact H;try easy;destr_hyps.
+	red in Hfair.
+	pinversion Hfair;subst. red in H7. specialize (H7 p q x2). 
+	eapply typ_path_preserves_fairness_helper with (xs:=cocons (M,l) ms) (ell:=x2). pfold. easy.
+	eapply H7;red. exists x1;easy.
+	right. eapply CIH with (xs:=ms). pinversion Hvalid;try eapply valid_path_mon;subst;try easy. pfold. constructor.
+	pinversion Hfair;subst. easy.
+	easy.
+Qed.
+	
+Definition extends_to_fair M := exists l xs, coseq_head xs = Some (M,l) /\ proc_valid_pathC xs /\ fair_path_proc xs.
+
+Definition fairness_feasible := forall M, extends_to_fair M.
+
+Lemma typ_path_exists: forall M gamma xs l, typ_sess M gamma -> proc_valid_pathC (cocons (M,l) xs) ->
+    exists ys,  typ_pathC (cocons (M,l) xs) ys
+    /\ local_valid_pathC ys /\ coseq_head ys= Some (gamma,l) .
+Proof.
+    intros * Hsess Hvalid.
+     exists (get_typ_path _ _ _ _ Hsess Hvalid). split;[|split];
+     try solve [eapply (get_typ_path_types) | eapply get_typ_path_valid].
+     pose proof Hvalid as Hvalid'.    
+    destruct l.
+    {
+        destruct l;pinversion Hvalid';subst;try apply valid_path_mon;try easy.
+    }
+    easy.
+Qed.
+
+
+Definition live_sess Mp := forall M, betaRtc Mp M -> (forall p q ell e P' M', p <>q -> unfoldP M ( (p <-- p_send q ell e P') ||| M') -> exists M'',
 betaRtc M ((p <-- P')|||M''))
 /\
-(forall p q llp M', unfoldP M ( (p <-- p_recv q llp) ||| M') -> exists M'' P' k,
+(forall p  q llp M', p <>q -> unfoldP M ( (p <-- p_recv q llp) ||| M') -> exists M'' P' k,
 onth k llp = Some P' /\
 betaRtc M ((p <-- P')|||M'')).
 
+Lemma path_to_betaRtc : forall xs M M' (lb:option label), coseq_head xs = Some (M,lb) -> 
+proc_valid_pathC xs ->
+eventually (fun u=> match u with cocons (a,_)_ => a=M' | _ => False end) xs ->
+	betaRtc M M'.
+Proof.
+	intros * Hhead Hvalid Hev.  generalize dependent lb. generalize dependent M. induction Hev.
+	destruct xs;try easy. destruct p;subst. intros. simpl in Hhead. inversion Hhead;subst. constructor 2.
+
+	intros. destruct x;try easy. simpl in Hhead. inversion Hhead;subst;clear Hhead.
+	pinversion Hvalid;try apply valid_path_mon;subst. inversion Hev;try easy.
+	specialize (IHHev H1 x).
+	econstructor 3 with (y:=x).
+	red in H3. destruct l;try easy. econstructor 1. exists (lcomm n n0 n1). easy.
+
+	eapply IHHev. simpl. reflexivity.
+Qed.
+
+Lemma sub_red_Rtc : forall M M' gamma, typ_sess M gamma -> betaRtc M M' -> exists gamma', typ_sess M' gamma'.
+Proof.
+	intros. generalize dependent gamma. induction H0.
+	intros. eapply sub_red in H0;try exact H. destr_hyps. exists x0;easy.
+	intros. exists gamma. easy.
+	intros. specialize (IHclos_refl_trans1 _ H). destr_hyps. 
+	eapply IHclos_refl_trans2;try exact H0.
+Qed.
+
+Ltac destruct_forallT := match goal with 
+                 | [ H: ForallT _ (?p <-- ?P)|- _] => inversion_clear H
+                | [ H: ForallT _ (?M ||| ?M' ) |- _] => inversion_clear H
+                end.
+
+Definition proc_path_head_is x (xs : coseq (session *option label)) := 
+        match xs with (cocons (M,_) _) => M = x
+        | _ => False
+        end.
+        Definition proc_path_head_unfolds_to_send p q (xs : coseq (session *option label)) := 
+        match xs with (cocons (M,_) _) => exists M' ell e P, unfoldP M ((p <-- p_send q ell e P) |||M')
+        | _ => False
+        end.
+        
+        Lemma betaP_lbl_invert : forall M M' p q ell gamma,
+        typ_sess M gamma -> betaP_lbl M (lcomm p q ell) M' ->
+        exists M'' P' llp e, unfoldP M ((p <-- p_send q ell e P' )|||(q <-- p_recv p llp) |||M'').
+        Proof.
+            intros * Hsess Hbeta.
+            generalize dependent gamma.
+            dependent induction Hbeta.
+            {
+                exists M, Q, xs, e. eauto with procs.
+            }
+            {
+                intros.
+                assert(Hsess2 : typ_sess M1' gamma).
+                {
+                    eapply typ_after_unfold in Hsess;try exact H;easy.
+                }
+                eapply IHHbeta in Hsess2 as IH_use;try reflexivity.
+                destr_hyps.
+                exists x, x0, x1, x2.
+                eauto with procs.
+            }
+        Qed.
+
+        Lemma betaP_lbl_send_unique : forall M M' M'' gamma p q ell ell' q', 
+        typ_sess M gamma ->
+        betaP_lbl M (lcomm p q ell) M' -> betaP_lbl M (lcomm p q' ell') M'' ->
+        q = q'.
+        Proof.
+            intros * Hsess Hbeta1 Hbeta2.
+            eapply betaP_lbl_invert in Hbeta1;try exact Hsess.
+            
+            eapply betaP_lbl_invert in Hbeta2;try exact Hsess.
+            destr_hyps.
+            eapply typ_after_unfold in H0 as Ht1;try exact Hsess.
+
+            eapply typ_after_unfold in H as Ht2;try exact Hsess.
+            inversion Ht1;inversion Ht2;subst.
+            
+            repeat destruct_forallT;destr_hyps.
+            assert(x9 =x7) by congruence;subst.
+            eapply inv_proc_send in H15, H19;try reflexivity.
+            destr_hyps. pinversion H28;subst;pinversion H26;subst;try apply sub_mon. easy.
+        Qed.
+
+Lemma proc_same_after_distinct_trans: 
+    forall M M' M'' p q p' q' ell ell' e P',
+    typable M ->
+    unfoldP M ((p<-- p_send q ell e P')|||M') ->
+    betaP_lbl M (lcomm p' q' ell') M'' ->
+    p' <> p -> q' <> p ->
+    exists M''' ell' e' P'', unfoldP M'' ((p<-- p_send q ell' e' P'')|||M''').
+    Proof.
+        intros * Htyp Hunf Hbeta Hpp Hqp.
+        destruct Htyp as [gamma Htyp].
+        eapply sub_red_strong_labelled in Hbeta as Hbeta';try exact Htyp;destr_hyps.
+        eapply lem_6_10 with (r:=p) in H0.
+        eapply typ_after_unfold in Hunf as Htyp';try exact Htyp. inversion Htyp';subst.
+        repeat destruct_forallT. destr_hyps.
+        eapply inv_proc_send in H7;try reflexivity;destr_hyps.
+        eapply betaP_lbl_invert in Hbeta;destr_hyps;try exact Htyp.
+        pinversion H11;subst;try apply sub_mon.
+        rewrite H4 in H0.
+        inversion H;subst.
+        eapply move_forward with (p:=p) in H as Hmf;
+        try solve [red;exists (ltt_send q ys);easy].
+        destr_hyps. eapply typ_after_unfold in H18 as Ht1;try exact H.
+        inversion Ht1;subst. repeat destruct_forallT. destr_hyps.
+        assert(x10= ltt_send q ys) by congruence;subst.
+        eapply typ_proc_inv_send in H27;try easy.
+        destr_hyps.
+        exists x8, x10, x12, x13.
+        eauto with procs.
+        red; intros;simpl;auto. simpl in H1. destruct H1;subst;try easy.
+    Qed.
+
+Lemma live_proc_helper2 : forall p q  xs,
+        p <> q ->
+        proc_valid_pathC xs ->
+        proc_path_head_unfolds_to_send p q xs -> 
+        weak_untilC ((fun u=> 
+        match u with | conil => True
+        | x => proc_path_head_unfolds_to_send p q x 
+         end)) 
+        (fun u=> exists ell', head_trans_proc p q ell' u) xs. 
+Proof.
+    intros * Hpq.  generalize dependent xs. pcofix CIH. 
+    intros * Hvalid Hphead. pfold.
+    destruct xs;try easy. destruct p0;try easy.
+    pinversion Hvalid;subst;try apply valid_path_mon.
+    {
+        econstructor 2. simpl in Hphead. destr_hyps. simpl. exists x, x0, x1, x2. easy. 
+        left.  
+        pfold. econstructor 3. easy.    
+    }
+    {
+        destruct l;try easy. red in H3.
+        destruct H3 as [Htab Htypable].
+        destruct (Nat.eq_dec n p);destruct (Nat.eq_dec n0 q);subst;try easy.
+        {
+            econstructor 1. simpl. exists n1; tauto.
+        }
+        {
+            simpl in Hphead.
+            Lemma unfold_beta_unique_send : 
+            forall M M' M'' p q ell e P' q' ell' gamma, typ_sess M gamma ->
+            unfoldP M ((p <-- p_send q ell e P')|||M'') ->
+            betaP_lbl M (lcomm p q' ell') M' -> q=q'.
+            Proof.
+                intros * Hsess Hunf Hbet.
+                eapply typ_after_unfold in Hsess as Hsess';try exact Hunf.
+                inversion Hsess';subst. repeat destruct_forallT. destr_hyps.
+                eapply inv_proc_send in H5;try reflexivity;destr_hyps.
+                eapply betaP_lbl_invert in Hbet as Hbinv;try exact Hsess.
+                destr_hyps.
+                eapply typ_after_unfold in Hsess as Hsess'';try exact H10.
+                inversion Hsess'';subst. repeat destruct_forallT. destr_hyps.
+                assert(x=x7) by congruence;subst.
+                eapply inv_proc_send in H18;try reflexivity;destr_hyps.
+                pinversion H24;pinversion H9;subst;try apply sub_mon;congruence. 
+            Qed.
+            red in Htypable. destr_hyps.
+            eapply unfold_beta_unique_send in Htab as Hunfq;try exact Hphead;
+            subst;try exact H0; try exact H;subst.
+            easy.
+        }
+        {
+            econstructor 2. easy.
+            right. eapply CIH;try easy.
+            simpl in Hphead. destr_hyps.  
+            eapply proc_same_after_distinct_trans in Htab as Hd;try exact H;try easy.
+        }
+        {
+            econstructor 2. easy.
+            right. eapply CIH;try easy.
+            simpl in Hphead. destr_hyps.  
+            eapply proc_same_after_distinct_trans in Htab as Hd;try exact H;try easy.
+            admit.
+        }
+    }
+Admitted.
+
+
+Lemma extends_to_fair_implies_live : fairness_feasible -> forall M gamma, typ_sess M gamma -> live_sess M.
+Proof. 
+	intros Ax_fairness * Hsess. red. intros. split.
+	{
+		intros * Hpq H0.
+		specialize (Ax_fairness M0). red in Ax_fairness. destr_hyps.
+		destruct x0;try easy. destruct p0;try easy. simpl in H1;inversion H1;subst;clear H1.
+		eapply sub_red_Rtc in Hsess;try exact H.
+		destruct Hsess as [gamma' Hsess].
+		eapply typ_path_exists in H2 as Htypp;try exact Hsess. destr_hyps.
+		assert(Hlive: liveCtx gamma').
+		{
+			Check liveness_global.
+            inversion Hsess;destr_hyps.
+			eapply liveness with (g:=x2);try easy. 
+            eapply assoc_implies_projectable in H12;try easy.  	
+		}
+        assert(Hlive_path: all_fair_live gamma').
+        {
+            eapply Hlive. constructor 2.   
+        }
+                    destruct x1;try easy. destruct p0. simpl in H5;inversion H5;subst;clear H5.
+
+        assert(Hev_local_trans: eventually (headComm p q) (cocons (gamma', x) x1)).
+        {
+            red in Hlive_path.
+            eapply typ_path_preserves_fairness in H3 as Hfair_local;try exact H1;try easy.
+            eapply Hlive_path in Hfair_local;try exact H4.
+            pinversion Hfair_local;subst. red in H7.
+            assert(exists s  xsp Tp', M.find p gamma' = Some (ltt_send q xsp) 
+            /\ onth ell xsp = Some (s,Tp')).
+            {
+                eapply typ_after_unfold in H0;try exact Hsess. inversion H0;subst. inversion_clear H10.
+                inversion_clear H11. destr_hyps.  
+                eapply inv_proc_send in H13;try reflexivity. destr_hyps. 
+                pose proof H17 as Hsub.
+                pinversion H17;subst;try apply sub_mon.
+                Search "sub" "inv" "send".
+                eapply subtype_send_inv in Hsub.
+                eapply Forall2R_prop with (l:=ell) (p:=(x4,x5)) in Hsub;
+                try solve [rewrite extendExtract;try easy]; tac_sanitize.
+                exists x7, ys, x9.
+                repeat split;try easy.
+            }
+            destr_hyps.
+            assert(tctxRE (lsend p q (Some x2) ell) gamma').
+            red. exists (m_update p x4 gamma').
+            eapply simple_red_send;try exact H6;try easy.
+            specialize (H7 p q x2 ell).
+            destr_hyps.
+            eapply H7. simpl. easy.
+        }
+        Check typ_path_preserves_fairness_helper.
+        Lemma live_proc_helper : forall p q xs ys, 
+        eventually (headComm p q) xs -> 
+        typ_pathC  ys xs -> exists ell,
+        eventually (head_trans_proc p q ell) ys.
+        Proof.
+            intros * Hev Htyp. generalize dependent ys. induction Hev.
+            {
+                intros. destruct xs;try easy. destruct p0. destruct o;try easy.
+                destruct l;try easy. simpl in H;destr_hyps;subst.
+                pinversion Htyp;subst. exists n1;simpl. constructor. easy. 
+            }
+            {
+                intros.
+                pinversion Htyp;subst. specialize (IHHev ms H3). 
+                destr_hyps. exists x. constructor 2. easy.   
+            }
+        Qed.
+        eapply live_proc_helper in Hev_local_trans as Hlpr;try exact H1.
+        destruct Hlpr as [ell' Hlpr].
+        eapply  live_proc_helper2 with (p:=p) (q:=q) in H2 as Hweak;try easy;
+        try solve [simpl; exists M', ell, e, P';  easy].
+        eapply weak_untilC_to_until in Hweak as Hunt;
+        try solve[
+        rewrite eventually_P_iff_P_suffix in Hlpr; destr_hyps;
+        rewrite eventually_P_iff_P_suffix; exists x2; split;try easy; exists ell'; easy].
+        eapply until_suf in Hunt.
+        destruct Hunt.
+        {
+            destr_hyps. destruct x;try easy. destruct l;try easy. simpl in H5;destr_hyps;subst.
+            pinversion H2;subst;try apply valid_path_mon. red in H9;destr_hyps.   
+        }
+        destruct xs.
+        eapply eventually_P_iff_P_suffix in Hev;destr_hyps.
+
+    }
 
